theories/reflect/progdef.v
@@ -8,62 +8,120 @@ From stdpp Require Import base strings gmap stringmap fin_maps.
 (* Not using iris but importing their ssreflect dependencies *)
 From iris.proofmode Require Import tactics.
 From shack Require Import lang progdef.
+From shack.reflect Require Import lang.
 
-Section SolveAcc.
-  (* assume a given set of class definitions *)
-  Context `{PDC: ProgDefContext}.
-
-  Fixpoint check_acc_def n c : bool :=
-    if n is S p then
-      if pdefs !! c is Some cdef then
-        if cdef.(superclass) is Some (parent, _) then
-          if pdefs !! parent is Some pdef then
-            check_acc_def p parent
-          else false
-        else true
+Fixpoint check_wf_ty (G : ProgDefContext) (ty : lang_ty) :=
+  match ty with
+  | BoolT
+  | DynamicT
+  | GenT _
+  | IntT
+  | MixedT
+  | NonNullT
+  | NothingT
+  | NullT
+  | SupportDynT
+  | ThisT => true
+  | ClassT _ t s =>
+      if pdefs !! t is Some cdef then
+      (length s =? length (generics cdef))%nat
+      && forallb (check_wf_ty G) s
       else false
+  | UnionT ty1 ty2 | InterT ty1 ty2 =>
+      check_wf_ty G ty1 && check_wf_ty G ty2
+  end.
+
+Lemma wf_ty_correct (G : ProgDefContext) (ty : lang_ty) :
+  check_wf_ty G ty -> wf_ty ty.
+Proof.
+  elim/lang_ty_ind: ty => //=.
+  - move=> ? tag s ih; case E: (_ !! _) => [cdef|] //.
+    case/andb_prop_elim=> hlen hwf; econstructor => //.
+    (* sigh... *)
+    + by rewrite -Nat.eqb_eq -Is_true_true.
+    + by move: hwf; rewrite forallb_True => /Forall_impl_in; apply.
+  - by move=> ty1 ty2 ih1 ih2 /andb_prop_elim[] {}/ih1 ih1 {}/ih2 ih2; constructor.
+  - by move=> ty1 ty2 ih1 ih2 /andb_prop_elim[] {}/ih1 ih1 {}/ih2 ih2; constructor.
+Qed.
+
+Definition check_wf_cdef_parent (G : ProgDefContext) (c : classDef) :=
+  if superclass c is Some (parent, σ) then
+       check_wf_ty G (ClassT true parent σ)
+    && forallb (check_generic_bounded (length (generics c))) σ
+    && forallb no_this σ
+  else true.
+
+Lemma wf_cdef_parent_correct (G : ProgDefContext) (c : classDef) :
+  check_wf_cdef_parent G c -> wf_cdef_parent c.
+Proof.
+  rewrite /check_wf_cdef_parent /wf_cdef_parent.
+  case: superclass => [[tag σ]|] //.
+  case/andb_prop_elim => /andb_prop_elim[] wfty wfs no_this; do! split.
+  - by apply: wf_ty_correct.
+  - by move/forallb_True/Forall_impl: wfs; apply; apply/generic_bounded_correct.  
+  - by move/forallb_True/Forall_impl: no_this; apply.
+Qed.
+
+Definition check_wf_cdef_parent_context (G : ProgDefContext) :=
+  forallb (fun kv => check_wf_cdef_parent G kv.2) (map_to_list pdefs).
+
+Lemma wf_cdef_parent_context_correct (G : ProgDefContext) :
+  check_wf_cdef_parent_context G -> map_Forall (λ _, wf_cdef_parent) pdefs.
+Proof.
+  rewrite /check_wf_cdef_parent_context map_Forall_to_list forallb_True.
+  by move/Forall_impl; apply => -[??] /=; apply/wf_cdef_parent_correct.
+Qed.
+
+Fixpoint check_acc_def (G: ProgDefContext) n c : bool :=
+  if n is S p then
+    if pdefs !! c is Some cdef then
+      if cdef.(superclass) is Some (parent, _) then
+        if pdefs !! parent is Some pdef then
+          check_acc_def G p parent
+        else false
+      else true
     else false
+  else false
 .
 
-  Lemma check_acc_def_correct n:
-    ∀ c, check_acc_def n c → Acc (λ x y, extends y x) c.
-  Proof.
-    elim: n => [ // | p ] /= hi c.
-    destruct (pdefs !! c) as [cdef | ] eqn:hcdef; last done.
-    destruct (cdef.(superclass)) as [ [parent ?] | ] eqn:hsuper; last first.
-    { move => _; constructor => ? h.
-      destruct h as [A B adef σ hadef' hsuper'].
-      by simplify_eq.
-    }
-    destruct (pdefs !! parent); last done.
-    move/hi => hacc.
-    constructor => ? h.
+Lemma check_acc_def_correct (G: ProgDefContext) n:
+  ∀ c, check_acc_def G n c → Acc (λ x y, extends y x) c.
+Proof.
+  elim: n => [ // | p ] /= hi c.
+  destruct (pdefs !! c) as [cdef | ] eqn:hcdef; last done.
+  destruct (cdef.(superclass)) as [ [parent ?] | ] eqn:hsuper; last first.
+  { move => _; constructor => ? h.
     destruct h as [A B adef σ hadef' hsuper'].
     by simplify_eq.
-  Qed.
+  }
+  destruct (pdefs !! parent); last done.
+  move/hi => hacc.
+  constructor => ? h.
+  destruct h as [A B adef σ hadef' hsuper'].
+  by simplify_eq.
+Qed.
 
-  Definition check_acc_defs n : bool :=
-    forallb (λ kv, check_acc_def n kv.1) (map_to_list pdefs).
+Definition check_acc_defs (G: ProgDefContext) n : bool :=
+  forallb (λ kv, check_acc_def G n kv.1) (map_to_list pdefs).
 
-  Lemma check_acc_defs_correct n:
-    check_acc_defs n →
-    ∀ c, Acc (λ x y, extends y x) c.
-  Proof.
-    assert (hForall:
-      check_acc_defs n → map_Forall (λ c _, Acc (λ x y, extends y x) c) pdefs).
-    { rewrite map_Forall_to_list /check_acc_defs forallb_True Forall_lookup.
-      rewrite Forall_lookup => h k [c cdef] hcdef /=.
-      apply check_acc_def_correct with n.
-      by apply h in hcdef.
-    }
-    move => h.
-    move: {hForall h} (hForall h).
-    rewrite map_Forall_lookup => h c.
-    destruct (pdefs !! c) as [cdef | ] eqn:hcdef; last first.
-    { constructor => ? hext.
-      destruct hext as [].
-      by simplify_eq.
-    }
+Lemma check_acc_defs_correct (G: ProgDefContext) n:
+  check_acc_defs G n →
+  ∀ c, Acc (λ x y, extends y x) c.
+Proof.
+  assert (hForall:
+    check_acc_defs G n → map_Forall (λ c _, Acc (λ x y, extends y x) c) pdefs).
+  { rewrite map_Forall_to_list /check_acc_defs forallb_True Forall_lookup.
+    rewrite Forall_lookup => h k [c cdef] hcdef /=.
+    apply check_acc_def_correct with n.
     by apply h in hcdef.
-  Qed.
-End SolveAcc.
+  }
+  move => h.
+  move: {hForall h} (hForall h).
+  rewrite map_Forall_lookup => h c.
+  destruct (pdefs !! c) as [cdef | ] eqn:hcdef; last first.
+  { constructor => ? hext.
+    destruct hext as [].
+    by simplify_eq.
+  }
+  by apply h in hcdef.
+Qed.
