theories/reflect/lang.v
@@ -1,0 +1,206 @@
+(*
+ * Copyright (c) Meta Platforms, Inc. and affiliates.
+ *
+ * This source code is licensed under the MIT license found in the
+ * LICENSE file in the root directory of this source tree.
+ *)
+From stdpp Require Import base strings gmap stringmap fin_maps.
+(* Not using iris but importing their ssreflect dependencies *)
+From iris.proofmode Require Import tactics.
+
+From shack Require Import lang progdef.
+
+Lemma Forall_impl_in {T : Type} (P Q : T → Prop) (l : list T) :
+  Forall P l → Forall (fun x => P x → Q x) l → Forall Q l.
+Proof.
+  elim: l => //= x l ih; rewrite !Forall_cons.
+  move=> [] Px Pl [] PQx /[dup] PQl /ih - /(_ Pl) Ql.
+  by split=> //; apply/PQx.
+Qed.
+
+Fixpoint check_generic_bounded (n : nat) (ty : lang_ty) :=
+  match ty with
+  | GenT k => (k <? n)%nat
+  | ClassT _ _ σ => forallb (check_generic_bounded n) σ
+  | UnionT s t
+  | InterT s t => check_generic_bounded n s && check_generic_bounded n t
+  | _ => true
+  end.
+
+Lemma generic_bounded_correct (n : nat) (ty : lang_ty) :
+  check_generic_bounded n ty → bounded n ty.
+Proof.
+  elim: ty => //=.
+  - move => ?? σ hi /forallb_True hb; constructor.
+    by apply: Forall_impl_in.
+  - move => s t hs ht /andb_prop_elim [h0 h1]; constructor; by firstorder.
+  - move => s t hs ht /andb_prop_elim [h0 h1]; constructor; by firstorder.
+  - move=> k lt_kn; constructor.
+    by rewrite -Nat.ltb_lt -Is_true_true.
+Qed.
+
+Fixpoint check_generic_bounded_expr n e :=
+  match e with
+  | BinOpE _ e1 e2 => check_generic_bounded_expr n e1 &&
+      check_generic_bounded_expr n e2
+  | UniOpE _ e => check_generic_bounded_expr n e
+  | UpcastE e ty => check_generic_bounded_expr n e &&
+      check_generic_bounded n ty
+  | _ => true
+  end.
+
+Lemma generic_bounded_expr_correct n e:
+  check_generic_bounded_expr n e →
+  expr_bounded n e.
+Proof.
+  elim : e => //=; try (intros; by constructor).
+  - move => ? e1 hi1 e2 hi2 /andb_prop_elim [h1 h2]; constructor; by firstorder.
+  - move => ? e hi h; constructor; by firstorder.
+  - move => e hi ty /andb_prop_elim [he hty]; constructor; first by firstorder.
+    by apply generic_bounded_correct.
+Qed.
+
+Fixpoint check_generic_bounded_cmd n cmd :=
+  match cmd with
+  | RuntimeCheckC _ _ c0 c1
+  | SeqC c0 c1 => check_generic_bounded_cmd n c0 &&
+      check_generic_bounded_cmd n c1
+  | GetC _ e _
+  | LetC _ e => check_generic_bounded_expr n e
+  | IfC cond c0 c1 => check_generic_bounded_expr n cond &&
+      check_generic_bounded_cmd n c0 &&
+      check_generic_bounded_cmd n c1
+  | CallC _ recv _ args =>
+      check_generic_bounded_expr n recv &&
+      forallb (λ kv, check_generic_bounded_expr n kv.2) (map_to_list args)
+  | NewC _ _ targs args =>
+      (if targs is Some σ then forallb (check_generic_bounded n) σ else true) &&
+      forallb (λ kv, check_generic_bounded_expr n kv.2) (map_to_list args)
+  | SetC recv _ rhs =>
+      check_generic_bounded_expr n recv &&
+      check_generic_bounded_expr n rhs
+  | SkipC
+  | ErrorC => true
+  end.
+
+Lemma generic_bounded_cmd_correct n cmd:
+  check_generic_bounded_cmd n cmd →
+  cmd_bounded n cmd.
+Proof.
+  elim : cmd => /=.
+  - move => _; by constructor.
+  - move => c0 hi0 c1 hi1 /andb_prop_elim [h0 h1]; constructor; by firstorder.
+  - move => ? e he; constructor; by apply generic_bounded_expr_correct.
+  - move => cond c0 hi0 c1 hi1 /andb_prop_elim [/andb_prop_elim [h0 h1]] h2.
+    constructor; try by firstorder.
+    by apply generic_bounded_expr_correct.
+  - move => ? e ? args /andb_prop_elim [he /forallb_True hargs]; constructor; first by apply generic_bounded_expr_correct.
+    rewrite map_Forall_to_list; apply: Forall_impl_in => //.
+    rewrite Forall_lookup => [? [? a]] /= h; by apply generic_bounded_expr_correct.
+  - move => ?? targs args /andb_prop_elim [h0 /forallb_True h1]; constructor.
+    + case: targs h0 => [σ | //] /forallb_True h; apply: Forall_impl_in => //.
+      rewrite Forall_lookup => k ty hk; by apply generic_bounded_correct.
+    + rewrite map_Forall_to_list; apply: Forall_impl_in => //.
+      rewrite Forall_lookup => [? [? a]] /= h; by apply generic_bounded_expr_correct.
+  - move => ? e ? he; constructor; by apply generic_bounded_expr_correct.
+  - move => recv ? rhs /andb_prop_elim [h0 h1]; constructor; by apply generic_bounded_expr_correct.
+  - move => ?? c0 hi0 c1 hi1 /andb_prop_elim [h0 h1]; constructor; by firstorder.
+  - move => _; by constructor.
+Qed.
+
+Definition check_wf_cdef_fields_bounded cdef :=
+  let n := length cdef.(generics) in
+  forallb (fun kv => check_generic_bounded n kv.2.2) (map_to_list cdef.(classfields)).
+
+Lemma wf_cdef_fields_bounded_correct cdef:
+  check_wf_cdef_fields_bounded cdef → wf_cdef_fields_bounded cdef.
+Proof.
+  rewrite /check_wf_cdef_fields_bounded /wf_cdef_fields_bounded /=.
+  move/forallb_True => hF; rewrite map_Forall_to_list; apply: Forall_impl_in => //.
+  rewrite Forall_lookup => ? [? [? ty]] /= ?; by apply generic_bounded_correct.
+Qed.
+
+Definition check_wf_cdef_fields_bounded_context (G: ProgDefContext) :=
+  forallb (fun kv => check_wf_cdef_fields_bounded kv.2) (map_to_list pdefs).
+
+Lemma wf_cdef_fields_bounded_context_correct (G: ProgDefContext):
+  check_wf_cdef_fields_bounded_context G →
+  map_Forall (λ _cname, wf_cdef_fields_bounded) pdefs.
+Proof.
+  rewrite /check_wf_cdef_fields_bounded_context forallb_True => hF.
+  rewrite map_Forall_to_list; apply: Forall_impl_in => //.
+  rewrite Forall_lookup => ? [? c] ? /=; by apply wf_cdef_fields_bounded_correct.
+Qed.
+
+Definition check_generic_bounded_mdef n mdef : bool :=
+  forallb (λ kv, check_generic_bounded n kv.2) (map_to_list mdef.(methodargs)) &&
+  check_generic_bounded n mdef.(methodrettype) &&
+  check_generic_bounded_cmd n mdef.(methodbody) &&
+  check_generic_bounded_expr n mdef.(methodret).
+
+Lemma generic_bounded_mdef_correct n mdef:
+  check_generic_bounded_mdef n mdef →
+  mdef_bounded n mdef.
+Proof.
+  rewrite /check_generic_bounded_mdef /mdef_bounded.
+  case/andb_prop_elim.
+  case/andb_prop_elim.
+  case/andb_prop_elim => /forallb_True h0 h1 h2 h3.
+  split.
+  { rewrite map_Forall_to_list; apply: Forall_impl_in => //=.
+    rewrite Forall_lookup => ? [? ty] /= ?; by apply generic_bounded_correct.
+  }
+  split; first by apply generic_bounded_correct.
+  split; first by apply generic_bounded_cmd_correct.
+  by apply generic_bounded_expr_correct.
+Qed.
+
+Definition check_cdef_methods_bounded cdef :=
+  let n := length cdef.(generics) in
+  forallb (fun kv => check_generic_bounded_mdef n kv.2) (map_to_list cdef.(classmethods)).
+
+Lemma cdef_methods_bounded_correct cdef:
+  check_cdef_methods_bounded cdef → cdef_methods_bounded cdef.
+Proof.
+  rewrite /check_cdef_methods_bounded /cdef_methods_bounded /=.
+  move/forallb_True => hF; rewrite map_Forall_to_list; apply: Forall_impl_in => //.
+  rewrite Forall_lookup => ? [? mdef] /= ?; by apply generic_bounded_mdef_correct.
+Qed.
+
+Definition check_cdef_methods_bounded_context (G: ProgDefContext) :=
+  forallb (fun kv => check_cdef_methods_bounded kv.2) (map_to_list pdefs).
+
+Lemma cdef_methods_bounded_context_correct (G: ProgDefContext):
+  check_cdef_methods_bounded_context G →
+  map_Forall (λ _cname, cdef_methods_bounded) pdefs.
+Proof.
+  rewrite /check_cdef_methods_bounded_context forallb_True => hF.
+  rewrite map_Forall_to_list; apply: Forall_impl_in => //.
+  rewrite Forall_lookup => ? [? c] ? /=; by apply cdef_methods_bounded_correct.
+Qed.
+
+Definition check_wf_cdef_constraints_bounded cdef : bool :=
+  let n := length cdef.(generics) in
+  forallb (λ c, check_generic_bounded n c.1 && check_generic_bounded n c.2) cdef.(constraints).
+
+Lemma wf_cdef_constraints_bounded_correct cdef:
+  check_wf_cdef_constraints_bounded cdef →
+  wf_cdef_constraints_bounded cdef.
+Proof.
+  rewrite /check_wf_cdef_constraints_bounded /wf_cdef_constraints_bounded forallb_True => hF.
+  apply: Forall_impl_in => //.
+  rewrite Forall_lookup => [? c1] ? /andb_prop_elim [h0 h1].
+  split; by apply generic_bounded_correct.
+Qed.
+
+Definition check_wf_cdef_constraints_bounded_context (G: ProgDefContext) : bool :=
+  forallb (fun kv => check_wf_cdef_constraints_bounded kv.2) (map_to_list pdefs).
+
+Lemma wf_cdef_constraints_bounded_context_correct (G: ProgDefContext) :
+  check_wf_cdef_constraints_bounded_context G →
+  map_Forall (λ _cname, wf_cdef_constraints_bounded) pdefs.
+Proof.
+  rewrite /check_wf_cdef_constraints_bounded_context forallb_True => hF.
+  rewrite map_Forall_to_list; apply: Forall_impl_in => //.
+  rewrite Forall_lookup => ? [? c] ? /=; by apply wf_cdef_constraints_bounded_correct.
+Qed.
